LeanChess.lean
@@ -1,4 +1,9 @@
 import domain.Game
+import domain.Command
+import domain.Clock
+import domain.Valid
+import domain.Mate
+import domain.Projection
 import domain.Deep
 import domain.Lazier
 import domain.Semantics
